# Logarithm Rules

### Product Rule `log(a*b) = log(a) + log(b)`

### Quotient Rule `log(a/b) = log(a) - log(b)`

### Power Rule `log(a^n) = n*log(a)`

### Change of Base Rule `log_a(b) = log_c(b) / log_c(a)`

This rule is used to change the base of a logarithm. It states that the logarithm of a number in base `a` is equal to the logarithm of the same number in base `c` divided by the logarithm of `a` in base `c`.

### Logarithmic Identity Rule `log_a(a) = 1`

### Logarithmic Inverse Rule `a^log_a(b) = b`

### Logarithm of One Rule `log_a(1) = 0`

### Logarithmic of Negative Number Rule `log_a(-b)` 

**is undefined** for any real number b and any base a that is a positive real number.

--------------------------------------